%% AMS-LaTeX Created by Wolfram Mathematica 7.0 : www.wolfram.com

\documentclass{article}
\usepackage{amsmath, amssymb, graphics}

\newcommand{\mathsym}[1]{{}}
\newcommand{\unicode}[1]{{}}

\begin{document}

\noindent\(\pmb{\{a>0,c>0,\text{gamma}>0\}}\)

\noindent\(\{a>0,c>0,\text{gamma}>0\}\)

\noindent\(\pmb{\text{f11} = -s_{-1}\text{==}a*y_{-2}}\)

\noindent\(-s_{-1}==a y_{-2}\)

\noindent\(\pmb{\text{f12} = -2*y_{-2}==x_{-2}*s_{-1}}\)

\noindent\(-2 y_{-2}==s_{-1} x_{-2}\)

\noindent\(\pmb{\text{f13} =-2*x_{-2}==y_{-2}*s_{-1} }\)

\noindent\(-2 x_{-2}==s_{-1} y_{-2}\)

\noindent\(\pmb{\left\{y_{-2},x_{-2},s_{-1}\right\}\text{/.}\text{Solve}\left[\{\text{f11},\text{f12},\text{f13}\},\left\{y_{-2},x_{-2},s_{-1}\right\}\right]}\)

\noindent\(\left\{\{0,0,0\},\left\{-\frac{2}{a},\frac{2}{a},2\right\},\left\{\frac{2}{a},\frac{2}{a},-2\right\}\right\}\)

\noindent\(\pmb{\text{f21}=0==a*y_{-1}}\)

\noindent\(0==a y_{-1}\)

\noindent\(\pmb{\text{f22}=-y_{-1}\text{==}-c*y_{-2}-x_{-2}*s_0-x_{-1}*s_{-1}}\)

\noindent\(-y_{-1}==-s_0 x_{-2}-s_{-1} x_{-1}-c y_{-2}\)

\noindent\(\pmb{\text{f23}=-x_{-1}\text{==}-c*x_{-2}+y_{-2}*s_0+y_{-1}*s_{-1}}\)

\noindent\(-x_{-1}==-c x_{-2}+s_0 y_{-2}+s_{-1} y_{-1}\)

\noindent\(\pmb{\text{sis}=\left\{y_{-1},x_{-1},s_0\right\}\text{/.}\text{Solve}\left[\{\text{f21},\text{f22},\text{f23}\},\left\{y_{-1},x_{-1},s_0\right\}\right]}\)

\noindent\(\pmb{\left\{\left\{0,-\frac{-c x_{-2}^2-c y_{-2}^2}{x_{-2}-s_{-1} y_{-2}},-\frac{-c s_{-1} x_{-2}-c y_{-2}}{-x_{-2}+s_{-1} y_{-2}}\right\}\right\}}\)

\noindent\(\left\{\left\{0,-\frac{-c x_{-2}^2-c y_{-2}^2}{x_{-2}-s_{-1} y_{-2}},-\frac{-c s_{-1} x_{-2}-c y_{-2}}{-x_{-2}+s_{-1} y_{-2}}\right\}\right\}\)

\noindent\(\pmb{z=\%\text{/.}\left\{y_{-2}\to 2/a,x_{-2}\to 2/a,s_{-1}\to -2\right\}}\)

\noindent\(\left\{\left\{0,\frac{4 c}{3 a},\frac{c}{3}\right\}\right\}\)

\noindent\(\pmb{\text{f31}=s_1==a*y_0+\text{gamma}}\\
\pmb{\text{f32}=0==-c*y_{-1}-s_{-1}-x_{-2}*s_1-x_{-1}*s_0-x_0*s_{-1}}\\
\pmb{\text{f33}=0==-c*x_{-1}+y_{-2}*s_1-y_{-1}*s_0-y_0*s_{-1}}\)

\noindent\(s_1==\text{gamma}+a y_0\)

\noindent\(0==-s_{-1}-s_1 x_{-2}-s_0 x_{-1}-s_{-1} x_0-c y_{-1}\)

\noindent\(0==-c x_{-1}+s_1 y_{-2}-s_0 y_{-1}-s_{-1} y_0\)

\noindent\(\pmb{r=\left\{y_0,x_0,s_1\right\}\text{/.}\text{Solve}\left[\{\text{f31},\text{f32},\text{f33}\},\left\{y_0,x_0,s_1\right\}\right]}\)

\noindent\(\left\{\left\{-\frac{-c x_{-1}+\text{gamma} y_{-2}-s_0 y_{-1}}{-s_{-1}+a y_{-2}},-\frac{s_{-1}+s_0 x_{-1}+c y_{-1}}{s_{-1}}+\frac{x_{-2}
\left(-\text{gamma} s_{-1}+a c x_{-1}+a s_0 y_{-1}\right)}{s_{-1} \left(s_{-1}-a y_{-2}\right)},-\frac{-\text{gamma} s_{-1}+a c x_{-1}+a s_0 y_{-1}}{s_{-1}-a
y_{-2}}\right\}\right\}\)

\noindent\(\pmb{z=\%\text{/.}\left\{y_{-2}\to 2/a,x_{-2}\to 2/a,s_{-1}\to -2,\right.}\\
\pmb{\left.y_{-1}\to 0,x_{-1}\to 4*c/(3*a), s_0\to c/3\right\}}\)

\noindent\(\left\{\left\{\frac{2 c^2-3 \text{gamma}}{6 a},-1+\frac{\frac{5 c^2}{9}+\frac{\text{gamma}}{2}}{a},\frac{1}{6} \left(2 c^2+3 \text{gamma}\right)\right\}\right\}\)

\noindent\(\pmb{\text{f41}=2*s_2==a*y_1}\)

\noindent\(2 s_2==a y_1\)

\noindent\(\pmb{\text{f42}=y_1\text{==}-c*y_0-s_0-s_2 *x_{-2}-s_1* x_{-1}-s_0* x_0+x_1*s_{-1}}\\
\pmb{\text{f43}=x_1\text{==}-c*x_0+s_2 *y_{-2}+s_1* y_{-1}+y_0* s_0+y_1*s_{-1}}\)

\noindent\(y_1==-s_0-s_2 x_{-2}-s_1 x_{-1}-s_0 x_0+s_{-1} x_1-c y_0\)

\noindent\(x_1==-c x_0+s_2 y_{-2}+s_1 y_{-1}+s_0 y_0+s_{-1} y_1\)

\noindent\(\pmb{v=\left\{y_1,x_1,s_2\right\}\text{/.}\text{Solve}\left[\{\text{f41},\text{f42},\text{f43}\},\left\{y_1,x_1,s_2\right\}\right]}\)

\noindent\(\left\{\left\{-\frac{2 \left(-s_0-s_1 x_{-1}-c s_{-1} x_0-s_0 x_0+s_{-1} s_1 y_{-1}-c y_0+s_{-1} s_0 y_0\right)}{-2+2 s_{-1}^2-a x_{-2}+a
s_{-1} y_{-2}},-\left(-2 s_{-1} s_0-2 s_{-1} s_1 x_{-1}-2 c x_0-2 s_{-1} s_0 x_0-a c x_{-2} x_0-a s_0 y_{-2}-a s_1 x_{-1} y_{-2}-a s_0 x_0 y_{-2}+2
s_1 y_{-1}+a s_1 x_{-2} y_{-1}-2 c s_{-1} y_0+2 s_0 y_0+a s_0 x_{-2} y_0-a c y_{-2} y_0\right)/\left(-2+2 s_{-1}^2-a x_{-2}+a s_{-1} y_{-2}\right),-\frac{a
\left(-s_0-s_1 x_{-1}-c s_{-1} x_0-s_0 x_0+s_{-1} s_1 y_{-1}-c y_0+s_{-1} s_0 y_0\right)}{-2+2 s_{-1}^2-a x_{-2}+a s_{-1} y_{-2}}\right\}\right\}\)

\noindent\(\pmb{z=\%\text{/.}\left\{y_{-2}\to 2/a,x_{-2}\to 2/a,s_{-1}\to -2,\right.}\\
\pmb{y_{-1}\to 0,x_{-1}\to 4*c/(3*a), s_0\to c/3,}\\
\pmb{\left.y_0\to y,x_0\text{-$>$}-1+\frac{\frac{5 c^2}{9}+\frac{\text{gamma}}{2}}{a},s_1\text{-$>$}\frac{1}{6} \left(2 c^2+3 \text{gamma}\right)\right\}}\)

\noindent\(\text{Power}\text{::}\text{infy}: \text{Infinite expression }\text{$\backslash $!$\backslash $($\backslash $*StyleBox[}\frac{1}{0}\text{,
$\texttt{"}$MT$\texttt{"}$]$\backslash $)}\text{ encountered.} \rangle\rangle \)

\noindent\(\text{Power}\text{::}\text{infy}: \text{Infinite expression }\text{$\backslash $!$\backslash $($\backslash $*StyleBox[}\frac{1}{0}\text{,
$\texttt{"}$MT$\texttt{"}$]$\backslash $)}\text{ encountered.} \rangle\rangle \)

\noindent\(\text{Power}\text{::}\text{infy}: \text{Infinite expression }\text{$\backslash $!$\backslash $($\backslash $*StyleBox[}\frac{1}{0}\text{,
$\texttt{"}$MT$\texttt{"}$]$\backslash $)}\text{ encountered.} \rangle\rangle \)

\noindent\(\text{General}\text{::}\text{stop}: \text{Further output of }\text{$\backslash $!$\backslash $($\backslash $*StyleBox[}\text{Power}\text{::}\text{infy}\text{,
$\texttt{"}$MT$\texttt{"}$]$\backslash $)}\text{ will be suppressed during this calculation.} \rangle\rangle \)

\noindent\(\{\{\text{ComplexInfinity},\text{ComplexInfinity},\text{ComplexInfinity}\}\}\)

\end{document}
